src/lowparse/LowParse.Spec.ListUpTo.fsti
@@ -1,0 +1,99 @@
+module LowParse.Spec.ListUpTo
+include LowParse.Spec.Base
+
+module L = FStar.List.Tot
+module Seq = FStar.Seq
+
+let negate_cond
+  (#t: Type)
+  (cond: (t -> Tot bool))
+  (x: t)
+: Tot bool
+= not (cond x)
+
+let refine_with_cond
+  (#t: Type)
+  (cond: (t -> Tot bool))
+: Tot Type
+= (x: t { cond x == true })
+
+let parse_list_up_to_t
+  (#t: Type)
+  (cond: (t -> Tot bool))
+: Tot Type0
+= list (refine_with_cond (negate_cond cond)) & refine_with_cond cond
+
+inline_for_extraction
+let parse_list_up_to_kind (k: parser_kind) : Tot (k' : parser_kind {k' `is_weaker_than` k }) = {
+  parser_kind_low = 0;
+  parser_kind_high = None;
+  parser_kind_subkind = k.parser_kind_subkind;
+  parser_kind_metadata = None;
+}
+
+let consumes_if_not_cond
+  (#k: parser_kind)
+  (#t: Type)
+  (cond: (t -> Tot bool))
+  (p: parser k t)
+: Tot Type
+= 
+    (b: bytes) ->
+    (x: t) ->
+    (consumed: consumed_length b) ->
+    Lemma
+    (requires (parse p b == Some (x, consumed) /\ (~ (cond x))))
+    (ensures (consumed > 0))
+
+val parse_list_up_to
+  (#k: parser_kind)
+  (#t: Type)
+  (cond: (t -> Tot bool))
+  (p: parser k t { k.parser_kind_subkind <> Some ParserConsumesAll })
+  (prf: consumes_if_not_cond cond p)
+: Tot (parser (parse_list_up_to_kind k) (parse_list_up_to_t cond))
+
+val parse_list_up_to_eq
+  (#k: parser_kind)
+  (#t: Type)
+  (cond: (t -> Tot bool))
+  (p: parser k t { k.parser_kind_subkind <> Some ParserConsumesAll })
+  (prf: consumes_if_not_cond cond p)
+  (b: bytes)
+: Lemma
+  (parse (parse_list_up_to cond p prf) b == (
+    match parse p b with
+    | None -> None
+    | Some (x, consumed) ->
+      if cond x
+      then Some (([], x), consumed)
+      else begin match parse (parse_list_up_to cond p prf) (Seq.slice b consumed (Seq.length b)) with
+      | None -> None
+      | Some ((y, z), consumed') -> Some ((x::y, z), consumed + consumed')
+      end
+  ))
+
+val serialize_list_up_to
+  (#k: parser_kind)
+  (#t: Type)
+  (cond: (t -> Tot bool))
+  (#p: parser k t)
+  (prf: consumes_if_not_cond cond p)
+  (s: serializer p { k.parser_kind_subkind == Some ParserStrong })
+: Tot (serializer (parse_list_up_to cond p prf))
+
+val serialize_list_up_to_eq
+  (#k: parser_kind)
+  (#t: Type)
+  (cond: (t -> Tot bool))
+  (#p: parser k t)
+  (prf: consumes_if_not_cond cond p)
+  (s: serializer p { k.parser_kind_subkind == Some ParserStrong })
+  (xy: parse_list_up_to_t cond)
+: Lemma
+  (serialize (serialize_list_up_to cond prf s) xy == (
+    let (l, z) = xy in
+    match l with
+    | [] -> serialize s z
+    | x :: y -> serialize s x `Seq.append` serialize (serialize_list_up_to cond prf s) (y, z)
+  ))
